Simplify bisim/sim defintions (only one def now)

Equiv/Equiv.v
@@ -1,13 +1,13 @@
-Require Import List Util paco2.
+Require Import List Util paco3.
 Require Export SmallStepRelations StateType.
 
 Set Implicit Arguments.
 Unset Printing Records.
 
-Class ProgramEquivalence S S' `{StateType S} `{StateType S'} :=
+Class ProgramEquivalence X S S' `{StateType S} `{StateType S'} :=
   {
-    progeq : (S -> S' -> Prop) -> S -> S' -> Prop;
-    progeq_mon : monotone2 progeq
+    progeq : (X -> S -> S' -> Prop) -> X -> S -> S' -> Prop;
+    progeq_mon : monotone3 progeq
   }.
 
-Arguments ProgramEquivalence S S' {H} {H0}.
+Arguments ProgramEquivalence X S S' {H} {H0}.
